theories/lifetime/derived.v
@@ -93,8 +93,8 @@ Lemma reborrow E P κ κ' :
   ↑lftN ⊆ E →
   lft_ctx ⊢ κ' ⊑ κ -∗ &{κ}P ={E}=∗ &{κ'}P ∗ ([†κ'] ={E}=∗  &{κ}P).
 Proof.
-  iIntros (?) "#LFT #H⊑ HP". iMod (bor_reborrow' with "LFT HP") as "[Hκ' H∋]".
-    done. (* by exists κ'.
+  iIntros (?) "#LFT #H⊑ HP". (* iMod (bor_rebor' with "LFT HP") as "[Hκ' H∋]".
+    done. by exists κ'.
   iDestruct (borrow_shorten with "[H⊑] Hκ'") as "$".
   { iApply lft_incl_lb. iSplit. done. iApply lft_incl_refl. }
   iIntros "!>Hκ'". iApply ("H∋" with "[Hκ']"). iApply lft_dead_or. auto.
